%SI 2014-09-05

\documentclass{article}

\usepackage[T1]{fontenc}
\usepackage[utf8]{inputenc}
\usepackage[swedish]{babel}
\usepackage{fullpage}
\usepackage{amssymb}
\usepackage{bussproofs}
\usepackage{amsmath}
\usepackage{graphicx}
\usepackage{verbatim}
\usepackage{tikz}
\let\emptyset\varnothing


\title{Supplemental Instructions}
\date{
      %Place date here!
     }

\begin{document}
\maketitle

\section*{1}
\begin{itemize}
    \item[a) ] $y' = - \frac{3x}{\sqrt{1-3x^2}}$
    \item[b) ] $-2 sin(x) cos(2 cos(x))$
    \item[c) ] $2(sin(2x) + cos(2x))$
\end{itemize}

\section*{2}
\begin{itemize}
    \item[a) ] 
    $2x + 2y y' = 0$ \\
    $2y y' = -2x$ \\
    $y' = \frac{-2x}{2y} = - \frac{x}{y}$
    
    \item[b) ]
    $3x^2 + 3y^2 y' = 1 + 2 y' $ \\
    $3x^2 - 1 = - 3y^2 y' + 2 y' $ \\    
    $3x^2 - 1 = y' ( 2 - 3y^2   ) $ \\  
    $\frac{3x^2 - 1}{ 2 - 3y^2  } = y'  $ \\
    
    
\end{itemize}
\section*{3}
\begin{itemize}
\item[a )] $y(x) = x^{2} \implies x(y) = \sqrt{y}$
\item[b )] $y(x) = 2^{x} \implies x(y) = \log_{2}{y}$
\item[c )] $y(x) = tan(x) \implies x(y) = \arctan{y}$
\item[d )] $y(x) = 1/x \implies x(y) = 1/y$
\end{itemize}

\section*{4}
$f(x) = x^2 \implies f^{-1}(x)=  \sqrt{x}$ \\
$f'(x) = 2x$ \\
$\frac{d}{dx} f^{-1}(x) = \frac{1}{f'(f^{-1}(x))}$
$\frac{d}{dx} \sqrt{x} = \frac{1}{f'(\sqrt{x})} = \frac{1}{2(\sqrt{x})}$
\section*{5}
\begin{itemize}
    \item[a) ] $3$
    \item[b) ] $2\sqrt{2}$
    \item[c) ] $1$
    \item[d) ] $x^5$
    \item[e) ] $ln \frac{64}{81}$
    \item[f) ] $x = \frac{ln(2)}{ln(2) - ln(3)}$
\end{itemize}

\section*{6}
\begin{itemize}
    \item[a) ] $e^x(x + 1) - 1$
    \item[b) ] $e^{x+e^{x}}$
    \item[c) ] $ln(x)$
\end{itemize}

\section*{7}
\begin{itemize}
    \item[a) ] $\frac{1}{\sqrt{-x^2 + x + 2}}$
    \item[b) ] $2x arctan(x) +1$
    \item[c) ] $arccos(x) - \frac{x}{\sqrt{1-x^2}}$
\end{itemize}

\end{document}
